Update parse table representation, give parser a more expressive return type

ExampleGrammars.v
@@ -2,10 +2,10 @@ Require Import Grammar.
 Require Import List.
 Import ListNotations.
 
-(* Grammar 3.11 from Appel's "Modern Compiler Implementation in ML" *)
+(* Grammar 3.11 from Appel's "Modern Compiler Implementation 
+   in ML" *)
 Definition g311 : grammar :=
-  [
-    (NT "S", [T "if"; NT "E"; T "then"; NT "S"; T "else"; NT "S"]);
+  [(NT "S", [T "if"; NT "E"; T "then"; NT "S"; T "else"; NT "S"]);
    (NT "S", [T "begin"; NT "S"; NT "L"]);
    (NT "S", [T "print"; NT "E"]);
   
@@ -14,7 +14,46 @@ Definition g311 : grammar :=
    
    (NT "E", [T "num"; T "=="; T "num"])].
 
-(* Grammar 3.12 from Appel's "Modern Compiler Implementation in ML" *)
+(* Inner maps for the Grammar 3.11 parse table *)
+
+Definition S_map :=
+  SymbolMap.add
+    (T "if")
+    [T "if"; NT "E"; T "then"; NT "S"; T "else"; NT "S"]
+    (SymbolMap.add
+       (T "begin")
+       [T "begin"; NT "S"; NT "L"]
+       (SymbolMap.add
+          (T "print")
+          [T "print"; NT "E"]
+          (SymbolMap.empty (list symbol)))).
+
+Definition L_map :=
+  SymbolMap.add
+    (T "end")
+    [T "end"]
+    (SymbolMap.add
+       (T ";")
+       [T ";"; NT "S"; NT "L"]
+       (SymbolMap.empty (list symbol))).
+
+Definition E_map :=
+  SymbolMap.add
+    (T "num")
+    [T "num"; T "=="; T "num"]
+    (SymbolMap.empty (list symbol)).
+
+Definition g311ParseTable :=
+  SymbolMap.add
+    (NT "S") S_map
+    (SymbolMap.add
+       (NT "L") L_map
+       (SymbolMap.add
+          (NT "E") E_map
+          (SymbolMap.empty (SymbolMap.t (list symbol))))).
+
+
+(* Grammar 3.12 from the same textbook *)
 Definition g312 : grammar :=
   [(NT "Z", [T "d"]); 
    (NT "Z", [NT "X"; NT "Y"; NT "Z"]);
