ParserTests.v
@@ -7,15 +7,27 @@ Require Import String.
 Import ListNotations.
 Open Scope string_scope.
 
-Definition input1 := ["if"; "num"; "=="; "num"; "then"; "print"; "num"; "=="; "num"; "else"; "print"; "num"; "=="; "num"].
-Definition parseTree1 := Node "S" [Leaf "if";
-                                   Node "E" [Leaf "num"; Leaf "=="; Leaf "num"];
-                                   Leaf "then";
-                                   Node "S" [Leaf "print";
-                                             Node "E" [Leaf "num"; Leaf "=="; Leaf "num"]];
-                                   Leaf "else";
-                                   Node "S" [Leaf "print";
-                                             Node "E" [Leaf "num"; Leaf "=="; Leaf "num"]]].
+Definition input1 :=
+  ["if"; "num"; "=="; "num"; "then";
+     "print"; "num"; "=="; "num";
+    "else";
+      "print"; "num"; "=="; "num"].
+Definition parseTree1 :=
+  Node "S"
+       [Leaf "if";
+        Node "E"
+             [Leaf "num"; Leaf "=="; Leaf "num"];
+        Leaf "then";
+        Node "S"
+             [Leaf "print";
+              Node "E"
+                   [Leaf "num"; Leaf "=="; Leaf "num"]];
+        Leaf "else";
+        Node "S"
+             [Leaf "print";
+              Node "E"
+                   [Leaf "num"; Leaf "=="; Leaf "num"]]].
 
-Example test1 : parse (mkParseTable g311 100) (NT "S") input1 100 = true.
+Example test1 :
+  parse g311ParseTable "S" input1 100 = Accept parseTree1.
 Proof. cbv. reflexivity. Defined.
